\input{preamble.tex}

\begin{document}

    \part{A First Course in General Relativity\cite{first-course-on-gr}}

    \chapter{Special Relativity}

    \section*{On ``Principle of relativity (Galileo)"}

    \subsection*{Galilean invariance}

    \href{https://en.wikipedia.org/wiki/Newton\%27s_laws_of_motion}{Newton's laws of motion} hold in all frames related
    to one another by a \href{https://en.wikipedia.org/wiki/Galilean\_transformation}{Galilean transformation}. In
    other words, all frames related to one another by such a transformation are inertial (meaning, Newton's equation of
    motion is valid in these frames).\cite{galilean-invariance} The proof has been given by the book on page 2.

    \section*{1.5 - Construction of the coordinates used by another observer}

    \subsection*{Why would the tangent of the angle is the speed in Fig. 1.2?}

    Suppose $\mathcal{O}$ and $\mathcal{\bar{O}}$ both start out at the same position where $\mathcal{\bar{O}}$
    moves along the $x$ at some speed. After $t_1$, observer $\mathcal{O}$ sees $\mathcal{\bar{O}}$ at position $x_1$:

    \[ \mathcal{\bar{O}}_1 = (x_1, t_1) \]

    Observer  $\mathcal{\bar{O}}$, however, still sees themself at $x = 0$:

    \[ \mathcal{\bar{O}}_1 = (0, t_1) \]

    By definition where ``$\bar{t}$ is the locus of events at constant $\bar{x} = 0$", $\bar{t}$ is the straight line
    that passes the origin and the $(x_1, t_1)$:

    \begin{tikzpicture}[scale=1.5]
        \draw[->] (-3,0) node[left] (w) {}--(5,0) node[right] (x) {x};
        \draw[->] (0,-3) node[below] (s) {}--(0,5) node[above] (t) {t};
        \draw[line width=.5pt] (.25,-.25) rectangle (-.25,.25) node (o) {};
        \draw[line width=.5] (o)--(135:1) node[above] () {$\mathcal{\bar{O}}_0$, $\mathcal{O}_0$};

        \draw[black,line width=2pt,->] (0,0)--(4,4) node[above] (t-bar) {{$\bar{t}$}};

        \draw[dashed,line width=.5] (3,0) node[below] (x1) {$x_1$} --(3,3);
        \draw[dashed,line width=.5] (0,3) node[left] (t1) {$t_1$} --(3,3);
        \draw[line width=.5pt] (2.75,3.25) rectangle (3.25,2.75) node (f) {};
        \draw (f) node[right] {$(x_1, t_1)$};

        \draw [blue,thick,domain=225:270] plot ({3 + cos(\x)}, {3 + sin(\x)}) node (speed) {};
        \draw (2.5, 1.8) node[right] (speed) {Tangent of this angle is $\bar{v}$};
    \end{tikzpicture}

    \section*{1.6 - Why $(\Delta x)^2 + (\Delta y)^2 + (\Delta z)^2 - (\Delta t)^2 = 0$ for two events in the same light beam?}

    Let's say, in a simplified 1D case, event $\mathcal{E} = (x_0, t_0)$ and $\mathcal{P} = (x_1, t_1)$.

    \[ (\Delta x)^2 - (\Delta t)^2 = (x_1 - x_0)^2 - (t_1 - t_0)^2 \]

    Since the speed of light is 1,

    \[ (x_1 - x_0)^2 - (t_1 - t_0)^2 = (x_1 - x_0)^2 - (t_1 \times 1 - t_0 \times 1)^2 = (x_1 - x_0)^2 - (x_1 - x_0)^2 = 0 \]

    \section*{Why do we have a 2nd term in equation 1.3 on p.10?}

    \begin{align}
        \Delta\bar{s}^2 &= \sum_{\alpha = 0}^3\sum_{\beta = 0}^3 \boldsymbol{M}_{\alpha\beta}\left(\Delta x^{\alpha}\right)\left(\Delta x^{\beta}\right) \\
        &= \sum_{\alpha = 0}^0\sum_{\beta = 0}^3 \boldsymbol{M}_{\alpha\beta}\left(\Delta x^{\alpha}\right)\left(\Delta x^{\beta}\right) + \sum_{\alpha = 0}^3\sum_{\beta = 0}^0 \boldsymbol{M}_{\alpha\beta}\left(\Delta x^{\alpha}\right)\left(\Delta x^{\beta}\right) + \sum_{\alpha = 1}^3\sum_{\beta = 1}^3 \boldsymbol{M}_{\alpha\beta}\left(\Delta x^{\alpha}\right)\left(\Delta x^{\beta}\right)
    \end{align}

    \bibliographystyle{plain}
    \nocite{*}
    \bibliography{refs}
\end{document}
